theories/WellFormed.v
@@ -82,44 +82,155 @@ continuations are never empty*)
 
 (*second condition more beefy of wellformedness*)
 
-  Definition rfree_rel := (role*role) -> ig_ty -> Prop.
+  Definition rfree_rel := role -> role -> ig_ty -> Prop.
   Inductive rcv_Free : rfree_rel :=
-  | rfree_end p q cG: rcv_Free (p,q) (ig_end cG)
+  | rfree_end p q cG: rcv_Free p q (ig_end cG)
   | rfree_send p q CONT:
     ( forall l Ty G, CONT l = Some (Ty, G) ->
-      rcv_Free (p,q) G ) ->
-    rcv_Free (p,q) (ig_msg None p q CONT)
+      rcv_Free p q G ) ->
+    rcv_Free p q (ig_msg None p q CONT)
   | rfree_diff p p' q q' o CONT:
     ( forall l Ty G, CONT l = Some (Ty, G) ->
-      rcv_Free (p,q) G ) ->
-    (p,q) != (p',q') ->
-    rcv_Free (p,q) (ig_msg o p' q' CONT)
+      rcv_Free p q G ) ->
+      (p != p') || (q != q') ->
+      rcv_Free p q (ig_msg o p' q' CONT)
   .
   Hint Constructors rcv_Free.
 
-  Definition RCV_Free G := (forall p q, rcv_Free (p,q) G).
+  Derive Inversion rcvFree_inv with (forall p q G, rcv_Free p q G) Sort Prop.
+
+  Definition RCV_Free G := (forall p q, rcv_Free p q G).
 
   Inductive well_Formed : ig_ty -> Prop :=
   | wform_end cG: well_Formed (ig_end cG)
   | wform_send p q CONT:
     ( forall l Ty G, CONT l = Some (Ty, G) -> well_Formed G ) ->
-    ( forall l Ty G, CONT l = Some (Ty, G) -> rcv_Free (p,q) G ) ->
+    ( forall l Ty G, CONT l = Some (Ty, G) -> rcv_Free p q G ) ->
     well_Formed (ig_msg None p q CONT)
   | wform_recv p q l CONT:
     ( forall l Ty G, CONT l = Some (Ty, G) -> well_Formed G ) ->
     well_Formed (ig_msg (Some l) p q CONT)
  .
 
+  Lemma wform_unr CG : well_Formed (rg_unr CG).
+  Proof.
+    case: CG=>[|F T C]/=; constructor =>//=; move=>l Ty G; 
+      case: (C l) =>[[MTy G'']|]//[_<-]; by constructor.
+  Qed.
+
+  Lemma rcvFree_cont F T F' T' C
+    : rcv_Free F T (ig_msg None F' T' C) -> 
+      forall L Ty G, C L = Some (Ty, G) -> rcv_Free F T G.
+  Proof.
+    elim/rcvFree_inv=>
+      [ //
+      | _ p q C' H _ _ [_ _ C_C']
+      | _ p p' q q' o C' H _ _ _ [_ _ _ C_C']
+      ]; by move: C_C' H=>->.
+  Qed.
+
+  Lemma rfree_unr F T CG : rcv_Free F T (rg_unr CG).
+  Proof.
+    case: CG=>[|F' T' C]//=; case: (boolP ((F == F') && (T == T'))).
+    + move=>/andP-[/eqP<-/eqP<-]; apply/rfree_send=> L Ty G.
+      by case: (C L)=>[[Ty' CG] [Ty_Ty' <-]|]//.
+    + rewrite negb_and=>NEQ; apply/rfree_diff=>// L Ty G.
+      by case: (C L)=>[[Ty' CG] [_ <-]|]//.
+  Qed.
+
+  Lemma rfree_step G G' a F T 
+    (a_F: subject a != F) (a_T: subject a != T)
+    : step a G G' ->
+      rcv_Free F T G ->
+      rcv_Free F T G'.
+  Proof.
+    move=>ST; elim/step_ind_str: ST a_F a_T
+      =>[ L F' T' C Ty G0 C_L
+        | L F' T' C Ty G0 C_L
+        | {}a F' T' C0 C1 a_F' a_T' dom_C0_C1 step_C0_C1 Ih
+        | {}a L F' T' C0 C1 a_T' dom_C0_C1 step_C0_C1 Ih
+        | {}a CG G0 step_a0_CG_G0 Ih
+        ]/= a_F a_T.
+      - elim/rcvFree_inv => _ //=;
+          first by move=>p q C' _ p_F q_T [/esym/eqP]; rewrite (negPf a_F).
+        move=> p p' q q' o C' H Neq p_F q_T [_ F_p' q_T' EC']  {p_F q_T p q o}.
+        move: F_p' q_T' Neq EC' H=>->->T_T' {q'} -> H {C'}.
+        by apply/rfree_diff=>//; rewrite eq_sym.
+      - elim/rcvFree_inv => _ //= p p' q q' o C' H Neq _ _ [_ p'_F' q'_T' C'_C] {p q}.
+        by move: p'_F' q'_T' C'_C Neq H =>->->->Neq /(_ _ _ _ C_L).
+      - move: Ih; case: (boolP ((F == F') && (T == T'))).
+        + move=>/andP-[/eqP<-/eqP<-] Ih /rcvFree_cont-H.
+          apply: rfree_send=> L Ty G'' C1_L.
+          move: (ex_intro (fun G''=>_) G'' C1_L)=>/dom_C0_C1-[G''' C0_L].
+          move: (H _ _ _ C0_L)=>RF_G'''; by apply: (Ih _ _ _ _ C0_L C1_L).
+        + rewrite negb_and=>NEQ Ih /rcvFree_cont-H.
+          apply:rfree_diff=>// L Ty G'' C1_L.
+          move: (ex_intro (fun G=>_) G'' C1_L)=>/dom_C0_C1-[G''' C0_L].
+          by apply/(Ih _ _ _ _ C0_L C1_L a_F a_T)/(H _ _ _ C0_L).
+      - elim/rcvFree_inv=>//= _ p p' q q' o C H NEQ _ _ [_ p'_F' q'_T' C_C0] {o p q}.
+        move: p'_F' q'_T' C_C0 NEQ H=>->->->NEQ H { p' q' C}.
+        apply: rfree_diff=>// L' Ty G'' C1_L'.
+        move: Ih=>[same_K [Ty' [G0 [G1 [C0_L [C1_L [ST /(_ a_F a_T)-Ih]]]]]]].
+        case: (boolP (L == L'))=>[/eqP-L_L'|L_L'].
+        + move: L_L' C1_L'=><-; rewrite C1_L=>[[Eq_Ty Eq_G]]. 
+          by move: Eq_G Eq_Ty Ih C0_L C1_L=>->->Ih /H/Ih-RF_G'' _.
+        + by apply/H/(same_K _ _ L_L')/C1_L'.
+      - move=>_; apply/(Ih a_F a_T)/rfree_unr.
+  Qed.
 
   Lemma wform_step a G G':
     well_Formed G -> step a G G' -> well_Formed G'.
   Proof.
-  Admitted.
+    move=>WF_G STEP;
+      elim/step_ind_str: STEP
+        =>[ L F T C Ty G0 C_L
+          | L F T C Ty G0 C_L
+          |{}a F T C0 C1 a_F a_T dom_C0_C1 step_C0_C1 Ih
+          |{}a L F T C0 C1 a_T dom_C0_C1 step_C0_C1 Ih
+          |{}a CG G0 step_a0_CG_G0 Ih
+          ] in WF_G *.
+    - case E: _ / WF_G => [//|F' T' C' Wf _|//].
+      move: E Wf=>[_ _ <-] Wf; by constructor.
+    - case E: _ / WF_G => [//|//|L' F' T' C' Wf].
+      by move: E Wf=>[_ _ _ <-] /(_ _ _ _ C_L).
+    - case E: _ / WF_G =>[//|F' T' C' Wf_G Rf_G|//].
+      move: E Wf_G Rf_G=>[<-<-<-] Wf_G Rf_G {F' T' C'}.
+      constructor.
+      + move=>L' Ty G'' C1_L'.
+        move: (ex_intro (fun G''=>_) G'' C1_L')=>/dom_C0_C1-[G0'' C0_L'].
+        by apply/(Ih _ _ _ _ C0_L' C1_L')/Wf_G/C0_L'.
+      + move=>L' Ty G'' C1_L'.
+        move: (ex_intro (fun G''=>_) G'' C1_L')=>/dom_C0_C1-[G0'' C0_L'].
+        apply/(rfree_step a_F a_T (step_C0_C1 _ _ _ _ C0_L' C1_L')).
+        by apply/Rf_G/C0_L'.
+    - case E: _ / WF_G =>[//|//|F' T' L' C' WF].
+      move: E WF=>[_ _ _ <-] WF {L' F' T'}.
+      move: Ih=>[same_L [Ty [G0 [G1 [C0_L [C1_L [ST Ih]]]]]]].
+      constructor=> L' Ty' G'' C1_L'; case: (boolP (L == L'))=>[/eqP-L_L'|].
+      + move: L_L' C1_L' =><-; rewrite C1_L => [[Ty_Ty' G1_G']].
+        by move: G1_G' => <-; apply/Ih/WF/C0_L.
+      + by move=> L_L'; apply/WF/(same_L _ _ L_L')/C1_L'.
+    - by apply/Ih/wform_unr.
+  Qed.
 
   Lemma wform_RCV_Free G: 
     RCV_Free G -> well_Formed G.
   Proof.
-  Admitted.
+    elim/ig_ty_ind2: G=>[CG _|ST FROM TO C Ih]; first by constructor.
+    move=> RF; have {}RF: forall L Ty G, C L = Some (Ty, G) -> RCV_Free G.
+    { move=> L Ty G H P Q; move: (RF P Q).
+      elim/rcvFree_inv=>// _.
+      - move=> P' Q' C' RF_C _ _ [_ _ _ C_C'].
+        move: C_C' RF_C=>->RF_C; by apply/RF_C/H.
+      - move=> P' P'' Q' Q'' O_L C' RF_C _ _ _ [_ _ _ C_C'].
+        move: C_C' RF_C=>->RF_C; by apply/RF_C/H.
+    }
+    case: ST=>[L|]; constructor=> L' Ty G; 
+      move: (RF L') (Ih L'); case E: (C L')=>[[Ty' G']|]//= RF_L' Ih_L' [_ <-].
+    + by apply/Ih_L'=> P Q; apply/(RF_L' Ty' G' erefl).
+    + by apply/Ih_L'=> P Q; apply/(RF_L' Ty' G' erefl).
+    + by apply/(RF_L' Ty' G' erefl).
+  Qed.
 
 (*The two following lemmas are now true by construction.
 I left them there as a reminder for now; to be removed later.*)
@@ -134,8 +245,5 @@ I left them there as a reminder for now; to be removed later.*)
   Proof.
   by move=> hp; apply: wform_RCV_Free; apply: (RCVFree_GUnroll hp).
   Qed.*)
-
-
-
 
 End WellFormed.
